backends/lean/Aeneas/Data/Coinductive/Spec.lean
@@ -2,3 +2,4 @@ module
 public import Aeneas.Data.Coinductive.Spec.Spec
 public import Aeneas.Data.Coinductive.Spec.SpecDerived
 import Aeneas.Data.Coinductive.Spec.Tests
+import Aeneas.Data.Coinductive.Spec.TotalTests
